theories/experimental/helping/offers.v
@@ -1,0 +1,113 @@
+(* ReLoC -- Relational logic for fine-grained concurrency *)
+(** Offers used to implement the stack with helping
+Based on the case study <https://iris-project.org/pdfs/2017-case-study-concurrent-stacks-with-helping.pdf> *)
+From iris.proofmode Require Import tactics.
+From iris.algebra Require Import excl.
+From reloc Require Export reloc.
+
+Definition mk_offer : val :=
+  λ: "v", ("v", ref #0).
+Definition revoke_offer : val :=
+  λ: "v", if: CAS (Snd "v") #0 #2 then SOME (Fst "v") else NONE.
+Definition take_offer : val :=
+  λ: "v", if: CAS (Snd "v") #0 #1 then SOME (Fst "v") else NONE.
+
+Definition offerR := exclR unitR.
+Class offerG Σ := { offer_inG :> inG Σ offerR }.
+Definition offerΣ : gFunctors := #[GFunctor offerR].
+Instance subG_offerΣ {Σ} : subG offerΣ Σ → offerG Σ.
+Proof. solve_inG. Qed.
+
+Section rules.
+  Context `{!relocG Σ, !offerG Σ}.
+
+  Definition offer_token γ := own γ (Excl ()).
+
+  Lemma offer_token_exclusive γ : offer_token γ -∗ offer_token γ -∗ False.
+  Proof. iIntros "H1 H2". iDestruct (own_valid_2 with "H1 H2") as %[]. Qed.
+
+  (** The offer invariant *)
+  Definition is_offer γ (l : loc) (P Q : iProp Σ) :=
+    (∃ (c : nat), l ↦ #c ∗
+        (⌜c = 0⌝ ∗ P
+       ∨ ⌜c = 1⌝ ∗ (Q ∨ offer_token γ)
+       ∨ ⌜c = 2⌝ ∗ offer_token γ))%I.
+
+  Lemma is_offer_exclusive γ1 γ2 l P1 Q1 P2 Q2 :
+    is_offer γ1 l P1 Q1 -∗ is_offer γ2 l P2 Q2 -∗ False.
+  Proof.
+    iDestruct 1 as (?) "[Hl1 _]". iDestruct 1 as (?) "[Hl2 _]".
+    iDestruct (gen_heap.mapsto_valid_2 with "Hl1 Hl2") as %?. contradiction.
+  Qed.
+
+  Lemma make_is_offer γ l P Q : l ↦ #0 -∗ P -∗ is_offer γ l P Q.
+  Proof. iIntros "Hl HP". iExists 0; by eauto with iFrame. Qed.
+
+  Lemma mk_offer_l K (v : val) t A :
+    (∀ γ l, (∀ P Q, P -∗ is_offer γ l P Q) -∗ offer_token γ -∗ REL fill K (of_val (v, #l)) << t : A) -∗
+    REL fill K (mk_offer v) << t : A.
+  Proof.
+    iIntros "Hcont". rel_rec_l. rel_alloc_l l as "Hl".
+    iMod (own_alloc (Excl ())) as (γ) "Hγ". done.
+    rel_pures_l. iApply ("Hcont" with "[Hl] Hγ").
+    iIntros (P Q) "HP". iExists 0; eauto with iFrame.
+  Qed.
+
+  Lemma take_offer_l γ E o v t A K P Q :
+    (|={⊤, E}=> ▷ is_offer γ o P Q ∗
+         ▷ ((is_offer γ o P Q -∗ REL fill K (of_val NONEV) << t @ E : A)
+            ∧ (P -∗ (Q -∗ is_offer γ o P Q) -∗ REL fill K (of_val $ SOMEV v) << t @ E : A))) -∗
+    REL fill K (take_offer (v, #o)%V) << t : A.
+  Proof.
+    iIntros "Hlog". rel_rec_l. rel_pures_l.
+    rel_cmpxchg_l_atomic.
+    iMod "Hlog" as "(Hoff & Hcont)".
+    rewrite {1}/is_offer. iDestruct "Hoff" as (c) "[Hl Hoff]".
+    iModIntro. iExists _. iFrame "Hl". iSplit.
+    - iIntros (?). iNext.
+      iDestruct "Hcont" as "[Hcont _]".
+      iIntros "Hl".
+      rel_pures_l. iApply ("Hcont" with "[-]").
+      iExists _; iFrame.
+    - iIntros (?). simplify_eq/=.
+      assert (c = 0%nat) as -> by lia. (* :) *)
+      iNext. iIntros "Hl".
+      iDestruct "Hoff" as "[[% HP] | [[% ?] | [% ?]]]"; [| congruence..].
+      rel_pures_l.
+      iDestruct "Hcont" as "[_ Hcont]".
+      iApply ("Hcont" with "HP [-]").
+      iIntros "HQ". rewrite /is_offer. iExists 1.
+      iFrame. iRight. iLeft. iSplit; eauto.
+  Qed.
+
+  Lemma wp_revoke_offer γ l E P Q (v : val) Φ :
+    offer_token γ -∗
+    ▷ (|={⊤, E}=> ▷ is_offer γ l P Q ∗
+        ▷ ((is_offer γ l P Q -∗ Q ={E, ⊤}=∗ Φ NONEV)
+           ∧ (is_offer γ l P Q -∗ P ={E, ⊤}=∗ Φ (SOMEV v)))) -∗
+    WP (revoke_offer (of_val (v, #l))) {{ Φ }}.
+  Proof.
+    iIntros "Hγ Hlog". wp_rec. wp_pures.
+    wp_bind (CmpXchg _ _ _). iApply wp_atomic.
+    iMod "Hlog" as "(Hoff & Hcont)".
+    rewrite {1}/is_offer. iDestruct "Hoff" as (c) "[Hl Hoff]".
+    iModIntro. iDestruct "Hoff" as "[(>-> & HP)|[(>-> & HQ) | (>-> & Htok)]]".
+    - wp_cmpxchg_suc; first fast_done.
+      iDestruct "Hcont" as "[_ Hcont]".
+      iMod ("Hcont" with "[-HP] HP") as "HΦ".
+      { iExists 2. iFrame "Hl". iRight. iRight. eauto. }
+      iModIntro. by wp_pures.
+    - wp_cmpxchg_fail; first done.
+      iDestruct "Hcont" as "[Hcont _]".
+      iDestruct "HQ" as "[HQ | Htok]"; last first.
+      { iExFalso. iApply (offer_token_exclusive with "Hγ Htok"). }
+      iMod ("Hcont" with "[-HQ] HQ") as "HΦ".
+      { iExists 1. iFrame "Hl". iRight. iLeft. eauto. }
+      iModIntro. by wp_pures.
+    - wp_cmpxchg_fail; first done.
+      iExFalso. iApply (offer_token_exclusive with "Hγ Htok").
+  Qed.
+
+End rules.
+
+Global Opaque offer_token is_offer revoke_offer take_offer mk_offer.
